src/proof/index.v
@@ -1,5 +1,5 @@
 From New.proof Require Import prelude empty_ffi.
-From New.proof Require Export apimodel list.
+From New.proof Require Export apimodel list util.
 From New.proof.kubernetes_model Require Export apimodel_init.
 
 Section proof.
@@ -51,12 +51,11 @@ Lemma wp_State__ByIndex_pod γ l kind index_name indexed_value
       "Hobjs_l" ∷ objs_l ↦* map (λ ptr, interface.mk (ptrT.id v1.Pod.id) #ptr) ptr_list ∗
       "Hptrs_purepods" ∷ ([∗ list] ptr;pure_pod ∈ ptr_list;pure_pod_list, ∃ pod, ptr ↦{dq} pod ∗ PurePod.deepown pod pure_pod dq) ∗
       "%Hwell_formed_pure_pod_list" ∷ ⌜ ∀ p, p ∈ pure_pod_list → PurePod.well_formed p ⌝ ∗
-      "%Hlen_size_eq" ∷ ⌜ length pure_pod_list = size pure_pod_map ⌝ ∗
       "%Hlist_in_map" ∷  ⌜ ∀ p, p ∈ pure_pod_list → pure_pod_map !! (PurePod.key p) = Some p ⌝ ∗
       "%Hmap_in_list" ∷ ⌜ ∀ k p, pure_pod_map !! k = Some p → p ∈ pure_pod_list ⌝ ∗
       "%Hown_pod_keys_eq" ∷ ⌜ ∀ key pod, pure_pod_map !! key = Some pod → key = PurePod.key pod ⌝ ∗
-      "%Hown_pod_list_namespace_eq" ∷ ⌜ ∀ key, key ∈ dom pure_pod_map → key.(KKey.Namespace') = parent_key.(KKey.Namespace') ⌝ ∗
       "%Hno_dup" ∷ ⌜ ∀ i j p1 p2, i ≠ j → pure_pod_list !! i = Some p1 → pure_pod_list !! j = Some p2 → (PurePod.key p1) ≠ (PurePod.key p2) ⌝ ∗
+      "%Hown_pod_list_namespace_eq" ∷ ⌜ ∀ key, key ∈ dom pure_pod_map → key.(KKey.Namespace') = parent_key.(KKey.Namespace') ⌝ ∗
       "Hown_parent" ∷ parent_key [[ γ.(γ_state) ]]↦ owned_parent ∗
       "Hown_pod_list" ∷ ([∗ map] key ↦ pod ∈ pure_pod_map, key [[ γ.(γ_state) ]]↦ PureKObject.Pod pod) ∗
       "Hown_child_keys" ∷ parent_key [[ γ.(γ_children) ]]↦ owned_child_keys
@@ -72,11 +71,11 @@ Proof.
   wp_auto.
   wp_apply (wp_State__objListLocked_pod with "[$Hown_pod_list $Hinv_Hstate_m_addr $Hinv_Hown_phys $Hinv_Hown_abs $Hinv_Hphys_abs_rep]").
   { iPureIntro. split; [done|]. destruct Hinv_Hghost_well_formed. done. }
-  iIntros (sl ptr_list pure_pod_list) "(Hsl & Hptr_pure_pod_list & %Hwell_formed & %Hlookup_abs
-    & %Hns_match & %Hmap_in_list & Hinv_Hstate_m_addr & Hinv_Hown_phys & Hinv_Hown_abs & Hinv_Hphys_abs_rep & Hown_pod_list)". wp_auto.
-  assert (∀ (k : KKey.t) (p : PurePod.t), pure_pod_map !! k = Some p → p ∈ pure_pod_list) as Hns_match'.
+  iIntros (sl ptr_list pure_pod_list) "(Hsl & Hlist & %Hwell_formed & %Hlookup_abs & %Hno_dup & %Hns_match & %Hmap_in_list &
+    Hinv_Hstate_m_addr & Hinv_Hown_phys & Hinv_Hown_abs & Hinv_Hphys_abs_rep & Hown_pod_list)". wp_auto.
+  assert (∀ (k : KKey.t) (p : PurePod.t), pure_pod_map !! k = Some p → p ∈ pure_pod_list) as Hmap_in_list'.
   { intros k p Hlookup. apply (Hmap_in_list k p Hlookup). unfold namespace_matches. left. done. }
-  clear Hns_match. rename Hns_match' into Hns_match.
+  clear Hns_match. rename Hmap_in_list' into Hns_match.
   set obj_list := map (λ ptr : loc, interface.mk (ptrT.id v1.Pod.id) (# ptr)) ptr_list.
   assert (length obj_list = length ptr_list) as Hlen_obj_ptr.
   { unfold obj_list. rewrite map_length. done. }
@@ -84,20 +83,20 @@ Proof.
   iPoseProof own_slice_cap_nil as "Hown_slice_nil_cap".
   iDestruct (own_slice_len with "Hsl") as %(Hsl_len1 & Hsl_len2).
   iDestruct (own_slice_wf with "Hsl") as %Hsl_cap.
-  iDestruct (big_sepL2_length with "Hptr_pure_pod_list") as %Hlen_ptr_pure_pod.
+  iDestruct (big_sepL2_length with "Hlist") as %Hlen_ptr_pure_pod.
   set P := (λ p, obj_has_controller_parent_of (PureKObject.Pod p) parent_key.(KKey.Kind') parent_key.(KKey.Name') (PureKObject.metadata owned_parent).(PureObjectMeta.UID')).
   set I := (∃ (i: w64) (val: interface.t) (sl': slice.t) (ptr_list': list loc) (pure_pod_list': list PurePod.t),
     "Hi_ptr" ∷ i_ptr ↦ i ∗
     "Hval_ptr" ∷ val_ptr ↦ val ∗
     "Hitems_ptr" ∷ items_ptr ↦ sl' ∗
     "Hsl'" ∷ sl' ↦* map (λ ptr : loc, interface.mk (ptrT.id v1.Pod.id) (# ptr)) ptr_list' ∗
-    "Hptr_pure_pod_list_pre" ∷ ([∗ list] ptr;pure_pod ∈ ptr_list';pure_pod_list', ∃ pod, PurePod.deepown_l ptr pod pure_pod 1) ∗
-    "Hptr_pure_pod_list_post" ∷ ([∗ list] ptr;pure_pod ∈ (drop (sint.nat i) ptr_list);(drop (sint.nat i) pure_pod_list), ∃ pod, PurePod.deepown_l ptr pod pure_pod 1) ∗
+    "Hlist_pre" ∷ ([∗ list] ptr;pure_pod ∈ ptr_list';pure_pod_list', ∃ pod, PurePod.deepown_l ptr pod pure_pod 1) ∗
+    "Hlist_post" ∷ ([∗ list] ptr;pure_pod ∈ (drop (sint.nat i) ptr_list);(drop (sint.nat i) pure_pod_list), ∃ pod, PurePod.deepown_l ptr pod pure_pod 1) ∗
     "Hcap_sl'" :: own_slice_cap interface.t sl' (DfracOwn 1) ∗
     "%Hfilter_ptr_list" ∷ ⌜ pure_pod_list' = filter P (take (sint.nat i) pure_pod_list) ⌝ ∗
     "%Hi" ∷ ⌜ 0 ≤ sint.Z i ≤ sint.Z (slice.len_f sl) ⌝
   )%I.
-  iAssert (I) with "[i val items Hptr_pure_pod_list]" as "Hloop_inv". {
+  iAssert (I) with "[i val items Hlist]" as "Hloop_inv". {
     iExists (W64 0), (default_val interface.t), (default_val slice.t), [], [].
     iFrame. iFrame "#". rewrite !big_sepL2_nil. done. }
   wp_for "Hloop_inv". wp_if_destruct.
@@ -108,7 +107,7 @@ Proof.
     { apply lookup_lt_is_Some_2. word. }
     assert (∃ this_pure_pod, pure_pod_list !! sint.nat i = Some this_pure_pod) as [this_pure_pod Hthis_pure_pod_lookup].
     { apply lookup_lt_is_Some_2. word. }
-    iPoseProof (big_sepL2_destruct_cons _ _ _ this_ptr this_pure_pod with "Hptr_pure_pod_list_post") as "[Hthis_ptr_pure_pod Hother_ptr_pure_pod]".
+    iPoseProof (big_sepL2_destruct_cons _ _ _ this_ptr this_pure_pod with "Hlist_post") as "[Hthis_ptr_pure_pod Hother_ptr_pure_pod]".
     { split. all: rewrite lookup_drop Nat.add_0_r; done. }
     iDestruct "Hthis_ptr_pure_pod" as (this_pod) "[Hthis_ptr Hdeepown_this_pod]".
     wp_apply (wp_index_of_podController with "[$Hthis_ptr $Hdeepown_this_pod]").
@@ -165,7 +164,7 @@ Proof.
         iIntros (sl'') "(Hsl'' & Hcap_sl'' & Hsl1)". wp_auto.
         wp_for_post.
         wp_for_post.
-        iAssert (I) with "[Hi_ptr Hval_ptr Hitems_ptr Hsl'' Hptr_pure_pod_list_pre Hthis_ptr Hdeepown_this_pod Hother_ptr_pure_pod Hcap_sl'']" as "Hloop_inv".
+        iAssert (I) with "[Hi_ptr Hval_ptr Hitems_ptr Hsl'' Hlist_pre Hthis_ptr Hdeepown_this_pod Hother_ptr_pure_pod Hcap_sl'']" as "Hloop_inv".
         { iExists (word.add i (W64 1)), this_obj, sl'', (ptr_list' ++ [this_ptr]), ((filter P (take (sint.nat i) pure_pod_list)) ++ [this_pure_pod]).
           assert (map (λ ptr : loc, interface.mk (ptrT.id v1.Pod.id) (# ptr)) ptr_list' ++ [this_obj] =
                   map (λ ptr, interface.mk (ptrT.id v1.Pod.id) (# ptr)) (ptr_list' ++ [this_ptr])) as ->.
@@ -189,16 +188,30 @@ Proof.
         rewrite bool_decide_false //.
         { destruct (bool_decide(this_pure_pod.(PurePod.ObjectMeta').(PureObjectMeta.Namespace') = parent_key.(KKey.Namespace'))) eqn:Hns.
           -- apply bool_decide_eq_true in Hns. rewrite <-Hns. intros Heq. apply HP. apply Hidx_val'. done.
-          -- destruct Hidx_val_prefix as [Hidx_val_prefix|Hidx_val_prefix].
-            ++ admit.
-            ++ admit. }
+          -- assert (slash_free (PureObjectMeta.Namespace' (PurePod.ObjectMeta' this_pure_pod))) as Hslash_free1.
+            { apply valid_namespace_slash_free.
+              assert (PurePod.well_formed this_pure_pod) as Hwf_pod.
+              { apply Hwell_formed. apply (list_elem_of_lookup_2 _ (sint.nat i)). done. }
+              destruct Hwf_pod as [Hwf_meta _]. unfold PureObjectMeta.well_formed in Hwf_meta. intuition. }
+            assert (slash_free (KKey.Namespace' parent_key)) as Hslash_free2.
+            { apply valid_namespace_slash_free.
+              destruct Hinv_Hghost_well_formed. 
+              pose proof Habs_state_well_formed parent_key owned_parent Hlookup_abs_parent as [Hparent_key Hwf_parent].
+              pose proof well_formed_object_has_well_formed_key parent_key owned_parent Hparent_key Hwf_parent as Hwf_key.
+              intuition. }
+            assert (PureObjectMeta.Namespace' (PurePod.ObjectMeta' this_pure_pod) ≠ KKey.Namespace' parent_key) as Hneq.
+            { intros H. apply bool_decide_eq_false in Hns. done. }
+            destruct Hidx_val_prefix as [Hidx_val_prefix|Hidx_val_prefix].
+            ++ rewrite Hidx_val_prefix. apply pod_controller_index_key_inequality1. all: done.
+            ++ destruct Hidx_val_prefix as [suffix Hidx_val_prefix]. rewrite Hidx_val_prefix.
+              apply pod_controller_index_key_inequality2. all: done. }
         wp_auto.
         wp_for_post.
         iAssert (I0) with "[Hj_ptr Hv_ptr Hitems_ptr Hsl' Hcap_sl']" as "Hloop_inv0".
         { iExists (word.add j (W64 1)), idx_val, sl'0. iFrame. iPureIntro. split;[|word]. intros. done. }
         iFrame.
     + wp_for_post.
-      iAssert (I) with "[Hi_ptr Hval_ptr Hitems_ptr Hsl' Hptr_pure_pod_list_pre Hthis_ptr Hdeepown_this_pod Hother_ptr_pure_pod Hcap_sl']" as "Hloop_inv".
+      iAssert (I) with "[Hi_ptr Hval_ptr Hitems_ptr Hsl' Hlist_pre Hthis_ptr Hdeepown_this_pod Hother_ptr_pure_pod Hcap_sl']" as "Hloop_inv".
       { iExists (word.add i (W64 1)), this_obj, sl'0, ptr_list', (filter P (take (sint.nat i) pure_pod_list)).
         iFrame.
         assert (sint.nat (word.add i (W64 1)) = S (sint.nat i)) as -> by word.
@@ -211,21 +224,47 @@ Proof.
         destruct (decide (P this_pure_pod)); [done|].
         rewrite filter_nil app_nil_r. done. }
       iFrame.
-  - iCombineNamed "Hinv_*" as "H".
+  - iAssert (⌜ ∀ key pod, pure_pod_map !! key = Some pod → abs_state !! key = Some (PureKObject.Pod pod) ⌝%I)
+    as "%Hsub_map".
+    { iAssert (⌜ fmap PureKObject.Pod pure_pod_map ⊆ abs_state ⌝%I) as %Hsubset.
+      { iApply (map_valid_subset with "Hinv_Hown_abs").
+        rewrite big_sepM_fmap. iFrame "Hown_pod_list". }
+      iPureIntro. intros key pod Hlookup.
+      assert ((fmap PureKObject.Pod pure_pod_map) !! key = Some (PureKObject.Pod pod)) as Hlookup_fmap.
+      { rewrite lookup_fmap. rewrite Hlookup. done. }
+      eapply lookup_weaken; [exact Hlookup_fmap|exact Hsubset]. }
+    iCombineNamed "Hinv_*" as "H".
     wp_apply (wp_Mutex__Unlock _ (kubernetes_inv γ l) with "[$Hown_Mutex H]").
     { iNamed "H". iFrame. iFrame "#". done. }
-    iApply "HΦ". iFrame "Hsl' Hptr_pure_pod_list_pre". iFrame.
+    iApply "HΦ". iFrame "Hsl' Hlist_pre". iFrame.
     iPureIntro.
     assert ((take (sint.nat i) pure_pod_list) = pure_pod_list) as ->.
     { apply take_ge. word. }
+    assert (∀ key pod, pure_pod_map !! key = Some pod → P pod) as HmapP.
+    { intros key pod Hlookup. destruct Hinv_Hghost_well_formed.
+      pose proof Hsub_map key pod Hlookup as Hlookup'.
+      assert (key ∈ (dom pure_pod_map)) as Hkeyin.
+      { apply elem_of_dom. exists pod. done. }
+      pose proof Hchildren_point_to_parent parent_key owned_parent key (PureKObject.Pod pod) (dom pure_pod_map)
+        Hlookup_abs_parent Hlookup' Hlookup_children as Hbi.
+      pose proof (proj1 Hbi) Hkeyin as Hobj_has_controller_parent_of. done. }
     split_and!.
     * intros p Hpin. apply Hwell_formed. apply list_elem_of_filter in Hpin. destruct Hpin as [_ Hpin]. done.
-    * admit.
-    * admit.
-    * admit.
-    * admit.
-    * admit.
-    * admit. 
-Admitted.
+    * intros p Hlookup_list. apply list_elem_of_filter in Hlookup_list as [HPp Hlookup_list].
+      pose proof Hlookup_abs p Hlookup_list as Hlookup_abs'.
+      destruct Hinv_Hghost_well_formed.
+      pose proof Hchildren_point_to_parent parent_key owned_parent (PurePod.key p) (PureKObject.Pod p)
+        (dom pure_pod_map) Hlookup_abs_parent Hlookup_abs' Hlookup_children as Hbi.
+      pose proof (proj2 Hbi) HPp as Hkey_in_dom. apply elem_of_dom in Hkey_in_dom as [p' Hlookup_map].
+      pose proof Hsub_map (PurePod.key p) p' Hlookup_map as Hlookup_abs''.
+      rewrite Hlookup_abs' in Hlookup_abs''. injection Hlookup_abs''. intros ->. done.
+    * intros k p Hlookup. pose proof HmapP k p Hlookup as HPp. apply list_elem_of_filter. split; [done|].
+      pose proof Hns_match k p Hlookup. done.
+    * intros k p Hlookup. destruct Hinv_Hghost_well_formed. pose proof Hsub_map k p Hlookup as Hlookup'.
+      pose proof Habs_state_well_formed k (PureKObject.Pod p) Hlookup' as Hwf. destruct Hwf as [Hwf _]. done.
+    * apply filter_preserves_key_uniqueness. done.
+    * intros k Hkindom. destruct Hinv_Hghost_well_formed. symmetry.
+      apply (Hparents_children_same_namespace _ (dom pure_pod_map)); [done|done].
+Qed.
 
 End proof.
